adapt nj_vs_hilbert.v to monad approach

nj_vs_hilbert.v
@@ -5,93 +5,20 @@ Require Import hilbert2nj nj2hilbert.
 
 Section NJvsH.
 
-Context { vatom : InfDecType } { tatom : Type } { fatom : Type }.
-Notation vfresh := (@fresh vatom).
-Notation vfresh_prop := (@fresh_prop vatom).
-Notation term := (@term vatom tatom).
-Notation closed t := (freevars t = nil).
-Notation tup := (@tup vatom tatom).
-Notation hterm := (@hterm vatom tatom).
-Notation hclosed t := (hfreevars t = nil).
-Notation formula := (@formula vatom tatom fatom).
-Notation hformula := (@hformula vatom tatom fatom).
-Notation n2h_term := (@n2h_term vatom tatom).
-Notation n2h_formula := (@n2h_formula vatom tatom fatom).
+Context { vatom : InfDecType } { tatom fatom : Type }.
+
+Arguments tvar {_} {_} {T} _.
+
+Notation hterm := (@term vatom tatom Empty_set).
+Notation hformula := (@formula vatom tatom fatom Nocon Icon Qcon Empty_set).
+Notation term := (@term vatom tatom nat).
+Notation formula := (@formula vatom tatom fatom Nocon Icon Qcon nat).
+Notation n2h_term r := (@tesubs vatom tatom nat Empty_set r).
+Notation n2h_formula r := (@esubs vatom tatom fatom Nocon Icon Qcon nat Empty_set r).
 Notation h2n_term := (@h2n_term vatom tatom).
 Notation h2n_formula := (@h2n_formula vatom tatom fatom).
 
-Hint Rewrite
-  (@tup_tup_com vatom tatom) (@tup_tsubs_com vatom tatom)
-  (@ntsubs_tup_com vatom tatom) (@ntsubs_z_tup vatom tatom)
-  (@freevars_tup vatom tatom) (@tsubs_tsubs_eq vatom tatom) : term_db.
-Hint Resolve (@closed_nofreevars vatom tatom) : term_db.
-Hint Rewrite (@freevars_ntsubs vatom tatom) using intuition; fail : term_db.
-Hint Rewrite (@nfree_tsubs vatom tatom)
-  using try (intuition; fail); (try apply closed_nofreevars); intuition; fail : term_db.
-Hint Rewrite (@ntsubs_tsubs_com vatom tatom)
-  using try (intuition; fail); (try apply closed_nofreevars); intuition; fail : term_db.
-Hint Rewrite (@tsubs_tsubs_com vatom tatom)
-  using try (intuition; fail); (try apply closed_nofreevars); intuition; fail : term_db.
-Hint Rewrite (@freevars_tsubs_closed vatom tatom)
-  using intuition; fail : term_db.
-
-Ltac formula_induction A :=
-  (try intros until A) ;
-  let XX := fresh "X" in
-  let xx := fresh "x" in
-  let A1 := fresh A in
-  let A2 := fresh A in
-  let ll := fresh "l" in
-  let lll := fresh "l" in
-  let tt := fresh "t" in
-  let IHll := fresh "IHl" in
-  induction A as [ XX ll | A1 ? A2 ? | xx A | xx A ]; simpl; intros;
-  [ rewrite ? flat_map_concat_map;
-    try f_equal; try (induction ll as [ | tt lll IHll ]; simpl; intuition;
-                      rewrite IHll; f_equal; intuition)
-  | try (f_equal; intuition)
-  | try (repeat case_analysis; intuition; f_equal; intuition; (rnow idtac); fail)
-  | try (repeat case_analysis; intuition; f_equal; intuition; (rnow idtac); fail) ];
-  try (now (rnow idtac)); try (now rcauto).
-
-Ltac term_induction t :=
-  (try intros until t);
-  let nn := fresh "n" in
-  let xx := fresh "x" in
-  let cc := fresh "c" in
-  let ll := fresh "l" in
-  let IHll := fresh "IHl" in
-  let i := fresh "i" in
-  let Hi := fresh "Hi" in
-  apply (term_ind_list_Forall t);
-  [ intros nn; try (now intuition); simpl
-  | intros xx; try (now intuition); simpl
-  | intros cc ll IHll; simpl;
-    rewrite ? flat_map_concat_map; rewrite ? map_map;
-    try f_equal;
-    try (apply map_ext_in; intros i Hi; specialize_Forall_all i);
-    try (apply Forall_forall; intros i Hi; specialize_Forall_all i);
-    try (now intuition) ];
-  try (now (rnow idtac)); try (now rcauto).
-
-Ltac hterm_induction t :=
-  (try intros until t);
-  let nn := fresh "n" in
-  let xx := fresh "x" in
-  let cc := fresh "c" in
-  let ll := fresh "l" in
-  let IHll := fresh "IHl" in
-  let i := fresh "i" in
-  let Hi := fresh "Hi" in
-  apply (hterm_ind_list_Forall t);
-  [ intros xx; try (now intuition); simpl
-  | intros cc ll IHll; simpl;
-    rewrite ? flat_map_concat_map; rewrite ? map_map;
-    try f_equal;
-    try (apply map_ext_in; intros i Hi; specialize_Forall_all i);
-    try (apply Forall_forall; intros i Hi; specialize_Forall_all i);
-    try (now intuition) ];
-  try (now (rnow idtac)); try (now rcauto).
+Hint Rewrite (@multi_tsubs_dvar vatom tatom) : term_db.
 
 
 (* * From Hilbert System to Natural Deduction *)
@@ -119,7 +46,7 @@ intros Hnd Hincl; inversion_clear Hnd; case_analysis; intros Hin; subst.
     exfalso; apply Heq; now inversion H4.
 Qed.
 
-Notation xf := (vfresh nil).
+Notation xf := (@fresh vatom nil).
 Definition vars_to_nat l :=
   ((fix f n s : list (vatom * nat) :=
     match s with
@@ -134,7 +61,7 @@ Proof. now induction l; intuition; simpl; f_equal. Qed.
 Lemma vars_to_nat_snd : forall l, map snd (vars_to_nat l) = rev (seq 0 (length l)).
 Proof. now induction l; intuition; simpl length; rewrite seq_S, rev_unit; simpl; f_equal. Qed.
 
-Lemma vars_to_nat_snd_NoDup : forall (A : hformula), NoDup (map snd (vars_to_nat (hffreevars A))).
+Lemma vars_to_nat_snd_NoDup : forall (A : hformula), NoDup (map snd (vars_to_nat (freevars A))).
 Proof. intros A; rewrite vars_to_nat_snd; apply NoDup_rev, NoDup_seq. Qed.
 
 Definition nthvar_nat l := fun n => nth (length l - S n) l xf.
@@ -157,16 +84,18 @@ destruct Hin as [Heq|Hin]; subst.
   apply IHl; now rewrite vars_to_nat_snd.
 Qed.
 
-Lemma ltgood_for_nthvar : forall t lv r lvn,
+Lemma no_tecapture_nthvar : forall t lv r lvn,
   (forall z, In z (map fst lvn) -> ~ In z lv) ->
   NoDup (map snd lvn) ->
   (forall i, In i (map snd lvn) -> In (r i, i) lvn) ->
-  ltgood_for (fun x : nat => hvar (r x)) lv (multi_tsubs (map (fun '(x, i) => (x, dvar i)) lvn) (h2n_term t)).
-Proof. hterm_induction t; intros lv r lvn Hlv Hnd Hincl.
-- revert Hnd Hincl Hlv; induction lvn; [ intros; reflexivity | destruct a; simpl; intros Hnd Hincl Hlv ].
-  case_analysis.
-  + rewrite multi_tsubs_closed; [ | reflexivity ]; simpl; f_equal.
-    apply Forall_forall; intros z Hz Heq; destruct Heq; intuition; subst.
+  no_tecapture_at (fun x => tvar (r x) : term) lv
+                  (multi_tsubs (map (fun '(x, i) => (x, dvar i)) lvn) (h2n_term t)).
+Proof. term_induction t.
+- intros lv r lvn Hlv Hnd Hincl.
+  revert Hnd Hincl Hlv; induction lvn;
+    [ intros; reflexivity | destruct a; simpl; intros Hnd Hincl Hlv ].
+  rnow case_analysis.
+  + apply Forall_forall; intros z Hz Heq; destruct Heq; intuition; subst.
     assert (Heq:= eq_refl n); eapply or_introl in Heq; apply Hincl in Heq.
     destruct Heq as [Heq|Hin].
     * inversion Heq; subst.
@@ -181,25 +110,26 @@ Proof. hterm_induction t; intros lv r lvn Hlv Hnd Hincl.
     * apply Hlv with z; intuition.
 - rewrite multi_tsubs_tconstr; simpl.
   apply Forall_fold_right, Forall_forall; intros u Hu.
-  rewrite map_map in Hu; apply in_map_iff in Hu; destruct Hu as [v [Heq Hin]]; subst.
+  rewrite map_map in Hu; apply in_map_iff in Hu; destruct Hu as [ v [Heq Hin] ]; subst.
   specialize_Forall IHl with v; apply IHl; intuition.
 Qed.
 
-Lemma lgood_for_nthvar : forall A lv r lvn,
+Lemma no_ecapture_nthvar : forall A lv r lvn,
   (forall z, In z (map fst lvn) -> ~ In z lv)->
   NoDup (map snd lvn) ->
   (forall i, In i (map snd lvn) -> In (r i, i) lvn) ->
-  lgood_for (fun x : nat => hvar (r x)) lv (multi_subs (map (fun '(x, i) => (x, dvar i)) lvn) (h2n_formula A)).
+  no_ecapture_at (fun x => tvar (r x) : term) lv
+                 (multi_subs (map (fun '(x, i) => (x, dvar i)) lvn) (h2n_formula A)).
 Proof. formula_induction A;
-  [ rewrite multi_subs_var | rewrite multi_subs_imp | rewrite multi_subs_frl | rewrite multi_subs_exs ];
+  [ rewrite multi_subs_fvar | rewrite multi_subs_fbin | rewrite multi_subs_fqtf ];
   simpl; f_equal; intuition.
 - apply Forall_fold_right, Forall_forall; intros t Ht.
-  rewrite map_map in Ht; apply in_map_iff in Ht; destruct Ht as [u [Heq Hu]]; subst.
-  apply ltgood_for_nthvar; intuition.
-- refine ?[mygoal]. Existential 1 := ?mygoal.
-  replace (remove_snd x (map (fun '(x0, i) => (x0, dvar i)) lvn))
+  rewrite map_map in Ht; apply in_map_iff in Ht; destruct Ht as [ u [Heq Hu] ]; subst.
+  apply no_tecapture_nthvar; intuition.
+- replace (remove_snd x (map (fun '(x0, i) => (x0, dvar i)) lvn))
      with (map (fun '(x0,i) => (x0, dvar i : term)) (remove_snd x lvn))
-    by (clear; induction lvn; intuition; unfold remove_snd; repeat case_analysis; f_equal; intuition).
+    by (clear; induction lvn; intuition; unfold remove_snd;
+        repeat case_analysis; f_equal; intuition).
   apply IHA.
   + intros z Hz Hinz.
     rewrite <- remove_snd_remove in Hz; apply in_remove in Hz.
@@ -212,13 +142,15 @@ Qed.
 Lemma hilbert_vs_nj_term : forall t r lvn,
   NoDup (map snd lvn) ->
   (forall i, In i (map snd lvn) -> In (r i, i) lvn) ->
-  n2h_term (fun x => hvar (r x)) (multi_tsubs (map (fun '(x,i) => (x, dvar i)) lvn) (h2n_term t)) = t.
-Proof. hterm_induction t; intros r lvn Hnd Hincl.
-- revert Hnd Hincl; induction lvn; [ intros; reflexivity | destruct a; simpl; intros Hnd Hincl ].
-  case_analysis.
-  + rewrite multi_tsubs_closed; [ | reflexivity ]; simpl; f_equal.
-    specialize Hincl with n.
-    assert (Heq := eq_refl n); eapply or_introl in Heq; apply Hincl in Heq; destruct Heq as [Heq|Heq].
+  n2h_term (fun x => tvar (r x))
+           (multi_tsubs (map (fun '(x,i) => (x, dvar i)) lvn) (h2n_term t)) = t.
+Proof. term_induction t.
+- intros r lvn Hnd Hincl.
+  revert Hnd Hincl; induction lvn; [ intros; reflexivity | destruct a; simpl; intros Hnd Hincl ].
+  rnow case_analysis.
+  + specialize Hincl with n.
+    assert (Heq := eq_refl n); eapply or_introl in Heq;
+      apply Hincl in Heq; destruct Heq as [Heq|Heq].
     * now inversion Heq; subst.
     * exfalso.
       inversion_clear Hnd; apply H.
@@ -236,16 +168,17 @@ Qed.
 Lemma hilbert_vs_nj_formula : forall A r lvn,
   NoDup (map snd lvn) ->
   (forall i, In i (map snd lvn) -> In (r i, i) lvn) ->
-  n2h_formula (fun x => hvar (r x)) (multi_subs (map (fun '(x,i) => (x, dvar i)) lvn) (h2n_formula A)) = A.
+  n2h_formula (fun x => tvar (r x))
+              (multi_subs (map (fun '(x,i) => (x, dvar i)) lvn) (h2n_formula A)) = A.
 Proof. formula_induction A;
-  [ rewrite multi_subs_var | rewrite multi_subs_imp | rewrite multi_subs_frl | rewrite multi_subs_exs ];
+  [ rewrite multi_subs_fvar | rewrite multi_subs_fbin | rewrite multi_subs_fqtf ];
   simpl; f_equal; intuition.
 - rewrite 2 map_map; rewrite <- (map_id l) at 2; apply map_ext_in; intros t Ht.
   now apply hilbert_vs_nj_term.
-- refine ?[mygoal]. Existential 1 := ?mygoal.
-  replace (remove_snd x (map (fun '(x0, i) => (x0, dvar i)) lvn))
+- replace (remove_snd x (map (fun '(x0, i) => (x0, dvar i)) lvn))
      with (map (fun '(x0,i) => (x0, dvar i : term)) (remove_snd x lvn))
-    by (clear; induction lvn; intuition; unfold remove_snd; repeat case_analysis; f_equal; intuition).
+    by (clear; induction lvn; intuition; unfold remove_snd;
+        repeat case_analysis; f_equal; intuition).
   apply IHA.
   + now apply NoDup_remove_snd.
   + intros i Hin; apply NoDup_remove_snd2; intuition.
@@ -255,24 +188,25 @@ Lemma hilbert_vs_nj : forall A,
   { L : _ & hprove A -> prove nil (multi_subs L (h2n_formula A))
           & prove nil (multi_subs L (h2n_formula A)) -> hprove A }.
 Proof.
-intros A; exists (map (fun '(x,i) => (x, dvar i)) (vars_to_nat (hffreevars A))); intros pi.
+intros A; exists (map (fun '(x,i) => (x, dvar i)) (vars_to_nat (freevars A))); intros pi.
 - apply h2n; intuition.
   + apply Forall_forall; intros t Ht.
     rewrite map_map in Ht.
-    now apply in_map_iff in Ht; destruct Ht as [u [Heq Hu]]; subst; destruct u; simpl.
+    now apply in_map_iff in Ht; destruct Ht as [ u [Heq Hu] ]; subst; destruct u; simpl.
   + intros z Hz.
     rewrite map_map; apply in_map_iff.
-    remember (hffreevars A) as l; revert z Hz; clear; induction l; intros z Hz; inversion_clear Hz; subst.
+    remember (freevars A) as l; revert z Hz; clear; induction l;
+      intros z Hz; inversion_clear Hz; subst.
     * exists (z, length l); split; simpl; intuition.
-    * apply IHl in H; destruct H as [(y,n) [Heq Hin]]; simpl in Heq; subst.
+    * apply IHl in H; destruct H as [ (y,n) [Heq Hin] ]; simpl in Heq; subst.
       exists (z, n); split; simpl; intuition.
-- apply n2h with (r:= fun x => hvar (nthvar_nat (hffreevars A) x)) in pi.
+- apply n2h with (r:= fun x => tvar (nthvar_nat (freevars A) x)) in pi.
   + simpl s2f in pi.
     rewrite hilbert_vs_nj_formula in pi; [ assumption | | ].
     * apply vars_to_nat_snd_NoDup.
     * apply vars_to_nat_content.
   + clear; repeat constructor.
-    apply lgood_for_nthvar; intuition.
+    apply no_ecapture_nthvar; intuition.
     * apply vars_to_nat_snd_NoDup.
     * now apply vars_to_nat_content.
 Qed.
@@ -280,22 +214,22 @@ Qed.
 
 (* * From Natural Deduction to Hilbert System *)
 
-Fixpoint freshvars_list l n :=
+Fixpoint freshvars_list (l : list vatom) n :=
   match n with
-  | 0 => vfresh l :: nil
-  | S k => let lv := freshvars_list l k in vfresh (lv ++ l) :: lv
+  | 0 => fresh l :: nil
+  | S k => let lv := freshvars_list l k in fresh (lv ++ l) :: lv
   end.
-Definition freshvars l n := hd (vfresh l) (freshvars_list l n).
-Definition freshterms l n := hvar (freshvars l n) : hterm.
+Definition freshvars l n := hd (fresh l) (freshvars_list l n).
+Definition freshterms l n := tvar (freshvars l n) : hterm.
 
 Lemma freshvars_list_fresh : forall l n x,
  In x (freshvars_list l n) -> ~ In x l.
 Proof.
 induction n; simpl; intros x Hin Hinl.
 - destruct Hin; intuition.
-  revert Hinl; subst; apply vfresh_prop.
+  revert Hinl; subst; apply fresh_prop.
 - destruct Hin; subst.
-  + apply vfresh_prop with (l := freshvars_list l n ++ l); in_solve.
+  + apply fresh_prop with (l0 := freshvars_list l n ++ l); in_solve.
   + now apply IHn in Hinl.
 Qed.
 
@@ -303,18 +237,19 @@ Lemma freshvars_list_prefix : forall l n m, n < m -> exists l',
   l' <> nil /\ freshvars_list l m = l' ++ freshvars_list l n.
 Proof. induction m; intros Hlt; [ lia | ].
 destruct (Nat.eq_dec n m); subst.
-- now exists (vfresh (freshvars_list l m ++ l) :: nil).
+- now exists (fresh (freshvars_list l m ++ l) :: nil).
 - assert (n < m) as Hlt2 by lia.
   apply IHm in Hlt2.
-  destruct Hlt2 as [l' [_ Heq]].
-  exists (vfresh (freshvars_list l m ++ l) :: l'); split ; [ | now rewrite <- app_comm_cons, <- Heq ].
+  destruct Hlt2 as [ l' [_ Heq] ].
+  exists (fresh (freshvars_list l m ++ l) :: l'); split ;
+    [ | now rewrite <- app_comm_cons, <- Heq ].
   intros Hnil; inversion Hnil.
 Qed.
 
 Lemma freshvars_list_NoDup : forall l n, NoDup (freshvars_list l n).
 Proof. induction n; simpl; constructor; intuition.
 - constructor.
-- apply vfresh_prop with (l := freshvars_list l n ++ l); in_solve.
+- apply fresh_prop with (l0 := freshvars_list l n ++ l); in_solve.
 Qed.
 
 Lemma freshvars_fresh : forall l n, ~ In (freshvars l n) l.
@@ -335,7 +270,7 @@ enough (forall n m, n < m -> freshvars l n = freshvars l m -> n = m) as Hlt.
   - assumption.
   - symmetry; now apply Hlt; [ lia | ]. }
 intros n m Hlt Heq; exfalso.
-apply freshvars_list_prefix with (l:= l) in Hlt; destruct Hlt as [l' [Hnil Hprf]].
+apply freshvars_list_prefix with (l:= l) in Hlt; destruct Hlt as [ l' [Hnil Hprf] ].
 unfold freshvars in Heq; rewrite Hprf in Heq.
 destruct l'; [ now apply Hnil | ]; simpl in Heq.
 destruct n; simpl in Heq, Hprf; rewrite Heq in Hprf.
@@ -347,32 +282,32 @@ destruct n; simpl in Heq, Hprf; rewrite Heq in Hprf.
   apply (freshvars_list_NoDup l m).
 Qed.
 
-Lemma ltgood_for_freshterms : forall t lv l, incl (l ++ freevars t) lv ->
-  ltgood_for (freshterms lv) l t.
-Proof. term_induction t; intros lv l' Hincl.
-- apply Forall_forall; intros x Hx; intuition; subst.
+Lemma no_tecapture_freshterms : forall t lv l, incl (l ++ tvars t) lv ->
+  no_tecapture_at (freshterms lv) l t.
+Proof. term_induction t.
+- intros lv l' Hincl.
+  apply Forall_forall; intros x Hx; intuition; subst.
   rewrite app_nil_r in Hincl; apply Hincl in Hx.
   revert Hx; apply freshvars_fresh.
 - apply Forall_fold_right, Forall_forall; intros u Hu.
   specialize_Forall IHl with u; apply IHl.
   intros z Hz.
-  apply Hincl; rewrite <- flat_map_concat_map.
+  apply H.
   apply in_or_app; apply in_app_or in Hz; destruct Hz as [Hz|Hz]; [left|right]; intuition.
   apply in_flat_map; exists u; intuition.
 Qed.
 
-Lemma lgood_for_freshterms : forall (A : formula) lv l, incl (l ++ allvars A) lv ->
-  lgood_for (freshterms lv) l A.
+Lemma no_ecapture_freshterms : forall (A : formula) lv l, incl (l ++ fvars A) lv ->
+  no_ecapture_at (freshterms lv) l A.
 Proof. formula_induction A.
 - apply Forall_fold_right, Forall_forall; intros t Ht.
-  apply ltgood_for_freshterms.
+  apply no_tecapture_freshterms.
   intros z Hz; apply H.
   apply in_or_app; apply in_app_or in Hz; destruct Hz as [Hz|Hz]; [left|right]; intuition.
   apply in_flat_map; exists t; intuition.
 - apply IHA1; intros z Hz; apply H; in_solve.
 - apply IHA2; intros z Hz; apply H; in_solve.
-- refine ?[mygoal]. Existential 1 := ?mygoal.
-  apply IHA; intros z Hz; apply H; in_solve.
+- apply IHA; intros z Hz; apply H; in_solve.
 Qed.
 
 Definition freshvars_to_nat l n :=
@@ -392,34 +327,37 @@ apply IHn.
 Qed.
 
 Lemma freshvars_to_nat_tcover : forall t lv n,
-  incl (freevars t) lv -> teigen_max t < n -> 
-  incl (hfreevars (n2h_term (freshterms lv) t)) (freevars t ++ map fst (freshvars_to_nat lv n)).
-Proof. term_induction t; intros lv k Hincl He z Hz.
-- inversion Hz; [ | inversion H]; subst.
+  incl (tvars t) lv -> teigen_max t < n -> 
+  incl (tvars (n2h_term (freshterms lv) t)) (tvars t ++ map fst (freshvars_to_nat lv n)).
+Proof. term_induction t.
+- intros lv k Hincl He z Hz.
+  inversion Hz; [ | inversion H]; subst.
   assert (In n (seq 0 k)) by (apply in_seq; lia).
   apply in_map with (f:= freshvars lv) in H.
   now rewrite freshvars_to_nat_fst, in_rev, rev_involutive.
-- rewrite flat_map_concat_map, map_map, <- flat_map_concat_map in Hz.
-  apply in_flat_map in Hz; destruct Hz as [u [Huin Hinu]].
+- intros z Hz.
+  rewrite <- flat_map_concat_map in Hz.
+  apply in_flat_map in Hz; destruct Hz as [ u [Huin Hinu] ].
   specialize_Forall IHl with u.
-  apply IHl with (n:= k) in Hinu.
+  apply IHl with (n:= n) in Hinu.
   + apply in_or_app; apply in_app_or in Hinu; destruct Hinu as [Hinu|Hinu]; [left| now right].
     rewrite <- flat_map_concat_map; apply in_flat_map; exists u; intuition.
   + intros y Hy.
-    apply Hincl.
-    rewrite <- flat_map_concat_map; apply in_flat_map; exists u; intuition.
-  + apply list_max_lt in He.
+    apply H.
+    apply in_flat_map; exists u; intuition.
+  + apply list_max_lt in H0.
     * apply in_map with (f:= teigen_max) in  Huin.
-      now specialize_Forall He with (teigen_max u).
+      now specialize_Forall H0 with (teigen_max u).
     * intros Heq.
       destruct l; inversion Huin; simpl in Heq; inversion Heq.
 Qed.
 
 Lemma freshvars_to_nat_cover : forall A lv n,
-  incl (allvars A) lv -> eigen_max A < n -> 
-  incl (hffreevars (n2h_formula (freshterms lv) A)) (ffreevars A ++ map fst (freshvars_to_nat lv n)).
+  incl (fvars A) lv -> eigen_max A < n -> 
+  incl (freevars (n2h_formula (freshterms lv) A)) (freevars A ++ map fst (freshvars_to_nat lv n)).
 Proof. formula_induction A; intros z Hz.
-- rewrite map_map, <- flat_map_concat_map in Hz; apply in_flat_map in Hz; destruct Hz as [t [Htin Hint]].
+- rewrite map_map, <- flat_map_concat_map in Hz;
+    apply in_flat_map in Hz; destruct Hz as [ t [Htin Hint] ].
   apply freshvars_to_nat_tcover with (t:= t) (n:= n) in Hint.
   + apply in_or_app; apply in_app_or in Hint; destruct Hint as [Hint|Hint]; [left| now right].
     rewrite <- flat_map_concat_map; apply in_flat_map; exists t; intuition.
@@ -434,8 +372,7 @@ Proof. formula_induction A; intros z Hz.
 - apply in_app_or in Hz; destruct Hz as [Hz|Hz].
   + apply IHA1 with (n:= n) in Hz; [ | intros y Hy; apply H | lia ]; try in_solve.
   + apply IHA2 with (n:= n) in Hz; [ | intros y Hy; apply H | lia ]; try in_solve.
-- refine ?[mygoal]. Existential 1 := ?mygoal.
-  apply in_remove in Hz; destruct Hz as [Hz Hneq].
+- apply in_remove in Hz; destruct Hz as [Hz Hneq].
   apply IHA with (n:= n) in Hz; intuition.
   + apply in_or_app; apply in_app_or in Hz; destruct Hz as [Hz|Hz]; [left| now right].
     now apply notin_remove.
@@ -443,10 +380,10 @@ Proof. formula_induction A; intros z Hz.
 Qed.
 
 Lemma nj_vs_hilbert_term : forall n lv t,
-  teigen_max t < n -> incl (freevars t) lv ->
+  teigen_max t < n -> incl (tvars t) lv ->
   multi_tsubs (freshvars_to_nat lv n) (h2n_term (n2h_term (freshterms lv) t)) = t.
-Proof. term_induction t; intros Hmax Hlv.
-- revert Hmax; clear; induction n; simpl; intros Hmax; try lia.
+Proof. term_induction t.
+- intros Hmax _; revert Hmax; clear; induction n; simpl; intros Hmax; try lia.
   rewrite freshvars_to_nat_S; simpl.
   destruct (Nat.eq_dec n0 n); subst.
   + rewrite eqb_refl; clear.
@@ -458,26 +395,26 @@ Proof. term_induction t; intros Hmax Hlv.
     * exfalso.
       apply n1; now apply freshvars_inj with (l:= lv).
     * apply IHn; lia.
-- assert (In x lv) as Hlv2 by (now apply Hlv; left).
+- intros Hmax Hlv.
+  assert (In x lv) as Hlv2 by (now apply Hlv; left).
   revert Hlv2; clear; induction n; simpl; intros Hlv; intuition.
   rewrite freshvars_to_nat_S; simpl; case_analysis; [ exfalso | intuition ].
   revert Hlv; apply freshvars_fresh.
 - rewrite multi_tsubs_tconstr; f_equal.
   rewrite map_map; rewrite <- (map_id l) at 2; apply map_ext_in; intros u Hu.
   specialize_Forall IHl with u; apply IHl.
-  + apply list_max_lt in Hmax.
+  + apply list_max_lt in H.
     * apply in_map with (f:= teigen_max) in Hu.
-      now specialize_Forall Hmax with (teigen_max u).
+      now specialize_Forall H with (teigen_max u).
     * intros Heq; destruct l; inversion Hu; simpl in Heq; inversion Heq.
-  + intros z Hz; apply Hlv; rewrite <- flat_map_concat_map; now apply in_flat_map; exists u.
+  + intros z Hz; apply H0; now apply in_flat_map; exists u.
 Qed.
 
 Lemma nj_vs_hilbert_formula : forall n lv A,
-  eigen_max A < n -> incl (allvars A) lv ->
+  eigen_max A < n -> incl (fvars A) lv ->
   multi_subs (freshvars_to_nat lv n) (h2n_formula (n2h_formula (freshterms lv) A)) = A.
 Proof. formula_induction A; 
-  [ rewrite multi_subs_var | rewrite multi_subs_imp | rewrite multi_subs_frl | rewrite multi_subs_exs ];
-  f_equal.
+  [ rewrite multi_subs_fvar | rewrite multi_subs_fbin | rewrite multi_subs_fqtf ]; f_equal.
 - rewrite 2 map_map; rewrite <- (map_id l) at 2; apply map_ext_in; intros t Ht.
   apply nj_vs_hilbert_term.
   + apply list_max_lt in H.
@@ -487,8 +424,7 @@ Proof. formula_induction A;
   + intros z Hz; apply H0; now apply in_flat_map; exists t.
 - apply IHA1; [ lia | intros z Hz; apply H0; in_solve ].
 - apply IHA2; [ lia | intros z Hz; apply H0; in_solve ].
-- refine ?[mygoal]. Existential 1 := ?mygoal.
-  enough (remove_snd x (freshvars_to_nat lv n) = freshvars_to_nat lv n) as Heq.
+- enough (remove_snd x (freshvars_to_nat lv n) = freshvars_to_nat lv n) as Heq.
   { rewrite Heq; apply IHA; intuition.
     intros z Hz; apply H0; in_solve. }
   assert (In x lv) as Hin by (apply H0; intuition).
@@ -497,22 +433,22 @@ Proof. formula_induction A;
   unfold freshvars_to_nat.
   rewrite seq_S, rev_unit; simpl.
   case_analysis; intuition.
-  +  exfalso; revert Hin; apply freshvars_fresh.
+  + exfalso; revert Hin; apply freshvars_fresh.
   + f_equal; destruct n; intuition.
 Qed.
 
-Lemma nj_vs_hilbert : forall A, ffreevars A = nil ->
+Lemma nj_vs_hilbert : forall A, freevars A = nil ->
   { r : _ & prove nil A -> hprove (n2h_formula r A)
           & hprove (n2h_formula r A) -> prove nil A }.
 (* closedness hypothesis required because of formulas like (∀x.∀y.P x) ⟶ P y *)
 Proof.
-intros A; exists (freshterms (allvars A)); intros pi.
+intros A; exists (freshterms (fvars A)); intros pi.
 - change A with (s2f nil A).
   apply n2h; intuition.
   simpl; repeat constructor.
-  apply lgood_for_freshterms.
+  apply no_ecapture_freshterms.
   intros z Hz; in_solve.
-- rewrite <- nj_vs_hilbert_formula with (S (eigen_max A)) (allvars A) _; [ | lia | now intros z Hz ].
+- rewrite <- nj_vs_hilbert_formula with (S (eigen_max A)) (fvars A) _; [ | lia | now intros z Hz ].
   apply h2n; intuition.
   + apply Forall_forall; intros t.
     remember (eigen_max A) as n; clear; induction n; simpl; intros Hin.
