hilbert2nj.v
@@ -4,57 +4,6 @@ Require Import stdlib_more.
 Require Export nj1 hilbert.
 
 
-Ltac term_induction t :=
-  (try intros until t);
-  let nn := fresh "n" in
-  let xx := fresh "x" in
-  let cc := fresh "c" in
-  let ll := fresh "l" in
-  let IHll := fresh "IHl" in
-  let i := fresh "i" in
-  let Hi := fresh "Hi" in
-  apply (term_ind_list_Forall t);
-  [ intros nn; try (now intuition); simpl
-  | intros xx; try (now intuition); simpl
-  | intros cc ll IHll; simpl; intros;
-    try (apply (f_equal (tconstr _)));
-    rewrite ? flat_map_concat_map, ? map_map;
-    try (apply (f_equal (@concat _)));
-    match goal with
-    | |- map _ ?l = ?l => rewrite <- (map_id l) at 2
-    | _ => idtac
-    end;
-    try (apply map_ext_in; intros i Hi; specialize_Forall_all i);
-    try (apply Forall_forall; intros i Hi; specialize_Forall_all i);
-    try (now intuition) ];
-  try (now (rnow idtac)); try (now rcauto).
-
-Ltac formula_induction A :=
-  (try intros until A) ;
-  let XX := fresh "X" in
-  let xx := fresh "x" in
-  let ncon := fresh "ncon" in
-  let bcon := fresh "bcon" in
-  let qcon := fresh "qcon" in
-  let A1 := fresh A in
-  let A2 := fresh A in
-  let ll := fresh "l" in
-  let lll := fresh "l" in
-  let tt := fresh "t" in
-  let IHll := fresh "IHl" in
-  induction A as [ XX ll | ncon | bcon A1 ? A2 ? | qcon xx A ]; simpl; intros;
-  [ rewrite ? flat_map_concat_map;
-    try (apply (f_equal (fvar _)));
-    try (induction ll as [ | tt lll IHll ]; simpl; intuition;
-         rewrite IHll; f_equal; intuition)
-  | try ((try f_equal); intuition; fail)
-  | try (apply (f_equal2 (fbin _)));
-    intuition
-  | (try apply (f_equal (fqtf _ _))); repeat case_analysis; try (intuition; fail); 
-     try (intuition; (rnow idtac); fail) ];
-  try (now (rnow idtac)); try (now rcauto).
-
-
 Section H2N.
 
 Context { vatom : DecType } { tatom fatom : Type }.
